Core/Term/BEq.lean
@@ -21,8 +21,7 @@ instance instLawfulBEq_CtorVariant : LawfulBEq Ctor0Variant where
 
 def Ctor1Variant.beq : Ctor1Variant -> Ctor1Variant -> Bool
 | sym, sym => true
-| fst, fst => true
-| snd, snd => true
+| prj n1, prj n2 => n1 == n2
 | appt a, appt b => a == b
 | _, _ => false
 
@@ -89,7 +88,7 @@ def Term.beq : Term -> Term -> Bool
 | tbind A1 K1 t1, tbind A2 K2 t2 => A1 == A2 && K1 == K2 && beq t1 t2
 | lam A1 t1, lam A2 t2 => A1 == A2 && beq t1 t2
 | guard a1 b1 c1, guard a2 b2 c2 => beq a1 a2 && beq b1 b2 && beq c1 c2
-| .mtch n1 a1 b1 c1 d1, .mtch n2 a2 b2 c2 d2 => true -- TODO: Fix
+-- | .mtch n1 a1 b1 c1 d1, .mtch n2 a2 b2 c2 d2 => true -- TODO: Fix
   -- if h : n1 = n2 then
   --   let c : Vect n1 Bool := λ i => beq (c1 i) (c2 (by rw [h] at i; exact i))
   --   let p : Vect n1 Bool := λ i => beq (b1 i) (b2 (by rw[h] at i; exact i))
